

Cheng Zhi Min A25CS0050

Gan Mei Lee A25CS0225

Ng Xuan Yee A25CS0291

$$1. (a) \begin{aligned} x^2 + x - 6 &= 0 \\ (x-2)(x+3) &= 0 \\ x &= -3, x = 2 \end{aligned}$$

$$\begin{aligned} A &= \{-3, 2\} \\ \therefore A' &= \{x \in \mathbb{Z} \mid x \neq -3, x \neq 2\} \end{aligned}$$

$$(b) (B-A) \cap C = \{1, 4\} \cap \{2, 3, 4\} = \{4\}.$$

$$(c) B \cap C = \{2, 4\} \\ n = 2$$

$$|P(B \cap C)| = 2^n = 2^2 = 4$$

$$\begin{aligned} 2. (((P \cup Q) \cap R)' \cup Q')' &= \cancel{((P \cup Q) \cap R) \cap Q} \text{ De Morgan} \\ &= (((P \cup Q) \cap R)')' \cap (Q')' \text{ (De Morgan's Law)} \\ &= ((P \cup Q) \cap R) \cap Q \text{ (Double Complement Law)} \\ &= Q \cap ((P \cup Q) \cap R) \text{ (Commutative Law)} \\ &= (Q \cap (P \cup Q)) \cap R \text{ (Associative Law)} \\ &= Q \cap R \text{ (Absorption Law)} \end{aligned}$$

3(a) $|A|$ = student in art class $|S|$ = student in science class

$$\begin{aligned} |A \cup S| &= |A| + |S| - |A \cap S| \\ &= 35 + 57 - 12 \\ &= 80 \end{aligned}$$

 $\therefore 80$ students

$$\begin{aligned} (b) |A \cup S| &= |A| + |S| + |A \cap S| \\ &= 35 + 57 \\ &= 92 \end{aligned}$$

 $\therefore 92$ students

4. (a) p : you try hard
 q : you have a talent
 r : you will get rich

$$(p \wedge q) \rightarrow r$$

(b) The statement false implies that r must be false and $(p \wedge q)$ must be true, because a statement $X \rightarrow Y$ is false when X is true and Y is false.

Since p is true (you try hard) and r is false, then q must be true as

$$(p \wedge q) \rightarrow r = (T \wedge T) \rightarrow F = T \rightarrow F = F.$$

\therefore You try hard and have a talent but you do not get rich.

(c) ~~r~~ r is true (you are rich)

Since r is true, the statement $(p \wedge q) \rightarrow r$ must be true, because a statement $X \rightarrow Y$ is ~~false~~ true whenever Y is true.

\therefore statement is true.

5.

p	q	r	$r \rightarrow p$	$q \wedge (r \rightarrow p)$	$p \vee (q \wedge (r \rightarrow p))$	A	$\sim p$	$q \rightarrow r$	B
F	F	F	T	F	F	T	T	T	T
F	F	T	F	F	F	T	T	T	T
F	T	F	T	T	T	F	T	F	F
F	T	T	F	F	F	T	T	T	T
T	F	F	T	F	T	F	F	T	F
T	F	T	T	F	T	F	F	T	F
T	T	F	T	T	T	F	F	F	F
T	T	T	T	T	T	F	F	T	F

$$\therefore A \equiv B$$

6. Assume x is odd and y is even.

Since x is odd, $x = 2h+1$ for some integer h and
since y is even, $y = 2k$ for some integer k .

$$x^2 - 2y = (2h+1)^2 - 2(2k)$$

$$= 4h^2 + 4h + 1 - 4k$$

$$= 2(2h^2 + 2h - 2k) + 1$$

$$= 2r + 1, \text{ where } r = 2h^2 + 2h - 2k \text{ and } r \in \mathbb{Z}$$

\therefore since $x^2 - 2y$ is in the form of $2r+1$ where r is an integer, so $x^2 - 2y$ is odd.

The statement is true and is proven.